clean up proofs with new match_letRecM_l tactic, prove no_errors_sum_2d

examples/arrays_proofs.v
@@ -16,26 +16,9 @@ Import arrays.
 
 Import VectorNotations.
 
-(* Print zero_array__tuple_fun. *)
-
-Definition zero_array_lrt
-  := LRT_Fun (SAWCorePrelude.bitvector 64)
-      (fun arg0 : SAWCorePrelude.bitvector 64 =>
-       LRT_Fun (BVVec 64 arg0 {_ : SAWCorePrelude.bitvector 64 & unit})
-         (fun _ : BVVec 64 arg0 {_ : SAWCorePrelude.bitvector 64 & unit} =>
-          LRT_Ret (BVVec 64 arg0 {_ : SAWCorePrelude.bitvector 64 & unit}))).
-
-Definition zero_array_letRec_lrt
-  := LRT_Fun (SAWCorePrelude.bitvector 64)
-      (fun arg0 : SAWCorePrelude.bitvector 64 =>
-       LRT_Fun (BVVec 64 arg0 {_ : SAWCorePrelude.bitvector 64 & unit})
-         (fun _ : BVVec 64 arg0 {_ : SAWCorePrelude.bitvector 64 & unit} =>
-          LRT_Fun {_ : SAWCorePrelude.bitvector 64 & unit}
-            (fun _ : {_ : SAWCorePrelude.bitvector 64 & unit} =>
-             LRT_Ret (BVVec 64 arg0 {_ : SAWCorePrelude.bitvector 64 & unit})))).
-
 Definition bvMem_lo := intToBv 64 0xf000000000000000.
 Definition bvMem_hi := intToBv 64 0x0fffffffffffffff.
+
 
 Definition zero_array_precond x
   := isBvsle 64 (intToBv 64 0) x /\ isBvsle 64 x bvMem_hi.
@@ -43,20 +26,14 @@ Definition zero_array_precond x
 Definition zero_array_invariant x x' (i : { _ & unit })
   := isBvsle 64 (intToBv 64 0) (projT1 i) /\ isBvsle 64 (projT1 i) x /\ x = x'.
 
-Definition zero_array_noErrors_letRec : lrtToType zero_array_lrt := fun x _ =>
-  assumingM (zero_array_precond x)
-   (letRecM (lrts:=LRT_Cons zero_array_letRec_lrt LRT_Nil)
-            (fun _ => (fun x' _ i => assumingM (zero_array_invariant x x' i)
-                                     noErrorsSpec, tt))
-            (fun _ => noErrorsSpec)).
-
 Lemma no_errors_zero_array
   : refinesFun zero_array (fun x _ => assumingM (zero_array_precond x) noErrorsSpec).
 Proof.
-  transitivity zero_array_noErrors_letRec; try reflexivity.
-  unfold zero_array, zero_array__tuple_fun, zero_array_noErrors_letRec, zero_array_letRec_lrt, zero_array_precond, zero_array_invariant, noErrorsSpec.
-  unfold bvultWithProof.
-  fold bvMem_lo; fold bvMem_hi.
+  unfold zero_array, zero_array__tuple_fun, zero_array_precond.
+  prove_refinement_match_letRecM_l.
+  - exact (fun a' _ i => assumingM (zero_array_invariant a a' i) noErrorsSpec).
+  unfold zero_array_invariant, noErrorsSpec.
+  unfold bvultWithProof; fold bvMem_lo; fold bvMem_hi.
   time "no_errors_zero_array" prove_refinement.
   (* A number of the remaining cases are covered exactly by hypotheses we already have in
      scope (e.g. proving the loop invariant holds initially). Note that `prove_refinement`
@@ -77,29 +54,9 @@ Proof.
     discriminate e_if0.
   - rewrite e_assuming4, e_assuming1 in e_if0.
     apply isBvslt_antirefl in e_if0; contradiction e_if0.
-  (* The remaining cases  are all
-     taken care of by either prove_refinement or assmption! *)
+  (* The remaining cases are all taken care of by either prove_refinement or assumption! *)
 Qed.
 
-
-Definition contains0_lrt
-  := LRT_Fun (bitvector 64)
-      (fun arg0 : bitvector 64 =>
-       LRT_Fun (BVVec 64 arg0 {_ : bitvector 64 & unit})
-         (fun _ : BVVec 64 arg0 {_ : bitvector 64 & unit} =>
-          LRT_Ret
-            (BVVec 64 arg0 {_ : bitvector 64 & unit} * ({_ : bitvector 64 & unit} * unit)))).
-
-Definition contains0_letRec_lrt
-  := LRT_Fun (bitvector 64)
-      (fun arg0 : bitvector 64 =>
-       LRT_Fun (BVVec 64 arg0 {_ : bitvector 64 & unit})
-         (fun _ : BVVec 64 arg0 {_ : bitvector 64 & unit} =>
-          LRT_Fun {_ : bitvector 64 & unit}
-            (fun _ : {_ : bitvector 64 & unit} =>
-             LRT_Ret
-               (BVVec 64 arg0 {_ : bitvector 64 & unit} *
-                ({_ : bitvector 64 & unit} * unit))))).
 
 Definition contains0_precond l
   := isBvsle 64 (intToBv 64 0) l /\ isBvsle 64 l bvMem_hi.
@@ -107,21 +64,15 @@ Definition contains0_precond l
 Definition contains0_invariant l l' (i : { _ & unit })
   := isBvsle 64 (intToBv 64 0) (projT1 i) /\ isBvsle 64 (projT1 i) l /\ l = l'.
 
-Definition contains0_noErrors_letRec : lrtToType contains0_lrt := fun x _ =>
-  assumingM (contains0_precond x)
-   (letRecM (lrts:=LRT_Cons contains0_letRec_lrt LRT_Nil)
-            (fun _ => (fun x' _ i => assumingM (contains0_invariant x x' i)
-                                     noErrorsSpec, tt))
-            (fun _ => noErrorsSpec)).
-
 (* This proof is *identical* to no_errors_zero_array except for in the one noted spot *)
 Lemma no_errors_contains0
   : refinesFun contains0 (fun x _ => assumingM (contains0_precond x) noErrorsSpec).
 Proof.
-  transitivity contains0_noErrors_letRec; try reflexivity.
-  unfold contains0, contains0__tuple_fun, contains0_noErrors_letRec, contains0_letRec_lrt, contains0_precond, contains0_invariant, noErrorsSpec.
-  unfold bvultWithProof.
-  unfold true, false; fold bvMem_lo; fold bvMem_hi.
+  unfold contains0, contains0__tuple_fun, contains0_precond.
+  prove_refinement_match_letRecM_l.
+  - exact (fun a' _ i => assumingM (contains0_invariant a a' i) noErrorsSpec).
+  unfold contains0_invariant, noErrorsSpec.
+  unfold bvultWithProof; fold bvMem_lo; fold bvMem_hi.
   time "no_errors_contains0" prove_refinement.
   all: try assumption.
   (* Different from no_errors_zero_array - this used to be taken care of by `prove_refinement`!
@@ -140,4 +91,53 @@ Proof.
     discriminate e_if0.
   - rewrite e_assuming4, e_assuming1 in e_if0.
     apply isBvslt_antirefl in e_if0; contradiction e_if0.
+Qed.
+
+
+Definition sum_2d_precond l1 l2
+  := isBvsle 64 (intToBv 64 0) l1 /\ isBvsle 64 l1 bvMem_hi /\
+     isBvsle 64 (intToBv 64 0) l2 /\ isBvsle 64 l2 bvMem_hi.
+
+Definition sum_2d_invariant1 (l1 l1' l2 l2' : bitvector 64) (i j : { _ & unit })
+  := isBvsle 64 (intToBv 64 0) (projT1 i) /\ isBvslt 64 (projT1 i) l1 /\ l1 = l1' /\
+     isBvsle 64 (intToBv 64 0) (projT1 j) /\ isBvsle 64 (projT1 j) l2 /\ l2 = l2'.
+
+Definition sum_2d_invariant2 (l1 l1' l2 l2' : bitvector 64) (i : { _ & unit })
+  := isBvsle 64 (intToBv 64 0) (projT1 i) /\ isBvsle 64 (projT1 i) l1 /\ l1 = l1' /\ l2 = l2'.
+
+Lemma no_errors_sum_2d
+  : refinesFun sum_2d (fun l1 l2 _ => assumingM (sum_2d_precond l1 l2) noErrorsSpec).
+Proof.
+  unfold sum_2d, sum_2d__tuple_fun, sum_2d_precond.
+  prove_refinement_match_letRecM_l.
+  - exact (fun a' a0' _ _ i j => assumingM (sum_2d_invariant1 a a' a0 a0' i j) noErrorsSpec).
+  - exact (fun a' a0' _ _ i => assumingM (sum_2d_invariant2 a a' a0 a0' i) noErrorsSpec).
+  unfold sum_2d_invariant1, sum_2d_invariant2, noErrorsSpec.
+  unfold bvultWithProof; fold bvMem_lo; fold bvMem_hi.
+  time "no_errors_sum_2d" prove_refinement.
+  all: try assumption.
+  * rewrite <- isBvult_to_isBvslt_pos, e_assuming5 in e_assuming6; try assumption.
+    rewrite e_assuming6 in e_maybe.
+    discriminate e_maybe.
+  * rewrite e_assuming7.
+    apply isBvsle_suc_r.
+    rewrite e_assuming8, e_assuming4.
+    reflexivity.
+  * rewrite <- e_assuming10 in e_if.
+    apply isBvslt_to_isBvsle_suc, isBvult_to_isBvslt_pos; assumption.
+  * rewrite <- e_assuming7 in e_if0.
+    vm_compute in e_if0; inversion e_if0.
+  * rewrite e_assuming8, e_assuming4 in e_if0.
+    vm_compute in e_if0; inversion e_if0.
+  * rewrite <- e_assuming3 in e_if0.
+    vm_compute in e_if0; inversion e_if0.
+  * rewrite e_assuming6, e_assuming2 in e_if0.
+    vm_compute in e_if0; inversion e_if0.
+  * rewrite e_assuming3.
+    apply isBvsle_suc_r, isBvslt_to_isBvsle.
+    rewrite e_assuming6, e_assuming2.
+    reflexivity.
+  * apply isBvslt_to_isBvsle_suc; assumption.
+  * rewrite <- e_assuming5 in e_if.
+    apply isBvult_to_isBvslt_pos; assumption.
 Qed.
