examples/loops_proofs.v
@@ -13,46 +13,26 @@ Import loops.
 
 Import SAWCorePrelude.
 
-Definition add_loop_lrt
-  := LRT_Fun {_ : bitvector 64 & unit}
-      (fun _ : {_ : bitvector 64 & unit} =>
-       LRT_Fun {_ : bitvector 64 & unit}
-         (fun _ : {_ : bitvector 64 & unit} =>
-            LRT_Ret {_ : bitvector 64 & unit})).
-
-Definition add_loop_letRec_lrt
-  := LRT_Fun {_ : bitvector 64 & unit}
-      (fun _ : {_ : bitvector 64 & unit} =>
-       LRT_Fun {_ : bitvector 64 & unit}
-         (fun _ : {_ : bitvector 64 & unit} =>
-          LRT_Fun {_ : bitvector 64 & unit}
-            (fun _ : {_ : bitvector 64 & unit} =>
-             LRT_Fun {_ : bitvector 64 & unit}
-               (fun _ : {_ : bitvector 64 & unit} =>
-                LRT_Ret {_ : bitvector 64 & unit})))).
-
 
 Lemma no_errors_add_loop : refinesFun add_loop (fun _ _ => noErrorsSpec).
 Proof.
-  transitivity ((fun _ _ => letRecM (lrts:=LRT_Cons add_loop_letRec_lrt LRT_Nil)
-                                    (fun _ => (fun _ _ _ _ => noErrorsSpec, tt))
-                                    (fun _ => noErrorsSpec)) : lrtToType add_loop_lrt);
-               try reflexivity.
-  unfold add_loop, add_loop__tuple_fun, add_loop_letRec_lrt, noErrorsSpec.
+  unfold add_loop, add_loop__tuple_fun.
+  prove_refinement_match_letRecM_l.
+  - exact (fun _ _ _ _ => noErrorsSpec).
+  unfold noErrorsSpec.
   time "no_errors_add_loop" prove_refinement.
 Qed.
 
 
-Definition add_loop_spec : lrtToType add_loop_lrt
-  := fun x y => returnM (existT _ (bvAdd 64 (projT1 x) (projT1 y)) tt).
+Definition add_loop_spec (x y : {_ : bitvector 64 & unit}) : CompM {_ : bitvector 64 & unit}
+  := returnM (existT _ (bvAdd 64 (projT1 x) (projT1 y)) tt).
 
 Lemma add_loop_spec_ref : refinesFun add_loop add_loop_spec.
 Proof.
-  transitivity (fun x y => letRecM (lrts:=LRT_Cons add_loop_letRec_lrt LRT_Nil)
-                                   (fun _ => (fun _ _ ret i => add_loop_spec ret i, tt))
-                                   (fun _ => add_loop_spec x y));
-               try reflexivity.
-  unfold add_loop, add_loop__tuple_fun, add_loop_spec, add_loop_letRec_lrt, noErrorsSpec.
+  unfold add_loop, add_loop__tuple_fun.
+  prove_refinement_match_letRecM_l.
+  - exact (fun _ _ ret i => add_loop_spec ret i).
+  unfold add_loop_spec.
   time "add_loop_spec_ref" prove_refinement.
   - f_equal.
     rewrite bvAdd_assoc.
